% 13_expand_simplify_brackets.tex

\question Expand brackets and simplify to solve.

\begin{multicols}{3}
\begin{parts}\Large
    \part $3(x + 2) = 2(3x + 6)$ \ms
    \part $2(5x + 1) = 4(3x + 4)$ \ms
    \part $3(2x - 2) = 4(x + 5)$ \ms
    \part $4(x + 3) = 2(3x + 5)$ \ms
    \part $5(x - 5) = 2(4x + 13)$ \ms
    \part $4(2x - 1) = 5(3x + 2)$ \ms
    \part $8(x - 1) = 2(3x + 7)$ \ms
    \part $3(x + 1) = 2(5x - 5)$ \ms
    \part $4(x - 1) = 2(3x + 4)$ \ms
    \part $2(3x - 4) = 4(x + 3)$ \ms
    \part $5(3x - 1) = 2(4x + 5)$ \ms
    \part $9x - 1 = 2(4x + 1)$ \ms
\end{parts}
\end{multicols} \ms
