\documentclass{beamer}

% Set up theme and colors
\usetheme{Madrid}
\setbeamercolor{structure}{fg=blue} % Use blue for headings and structure
\usepackage{amsmath} % For equation arrays

\title{Homework Solutions: Elimination Method}
\author{}
\date{}

\begin{document}

% Title Slide
\begin{frame}
    \titlepage
\end{frame}

% Slide 1: Solution to Question 1
\begin{frame}{Solution to Question 1}
Solve the system of equations:
\[
\begin{aligned}
    x + 5y &= 2 \\
    -x + 4y &= 3
\end{aligned}
\]
Steps:
\[
\begin{aligned}
    \text{Step 1: Add the two equations to eliminate } x: \\
    (x + 5y) + (-x + 4y) &= 2 + 3 \\
    9y &= 5 \quad \Rightarrow \quad y = 3
\end{aligned}
\]
\[
\begin{aligned}
    \text{Step 2: Substitute } y = 3 \text{ into the first equation:} \\
    x + 5(3) &= 2 \\
    x + 15 &= 2 \\
    x &= 2 - 15 \\
    x &= -13
\end{aligned}
\]
\[
(x, y) = (-13, 3)
\]
\end{frame}

% Slide 2: Solution to Question 2
\begin{frame}{Solution to Question 2}
Solve the system of equations:
\[
\begin{aligned}
    4x + 5y &= 1 \\
    x - y &= -2
\end{aligned}
\]
Steps:
\[
\begin{aligned}
    \text{Step 1: Multiply the second equation by 4 to align with the } x \text{-term:} \\
    \times 4 \quad (x - y &= -2) \\
    4x - 4y &= -8
\end{aligned}
\]
\[
\begin{aligned}
    \text{Step 2: Subtract the second equation from the first to eliminate } x: \\
    (4x + 5y) - (4x - 4y) &= 1 - (-8) \\
    9y &= 9 \quad \Rightarrow \quad y = 1
\end{aligned}
\]
\[
\begin{aligned}
    \text{Step 3: Substitute } y = 1 \text{ into the second original equation:} \\
    x - (1) &= -2 \\
    x &= -1
\end{aligned}
\]
\[
(x, y) = (-1, 1)
\]
\end{frame}

\end{document}
